src/Attestation_Session.v
@@ -1,0 +1,53 @@
+Require Import Maps Term_Defs_Core Manifest_Admits.
+Require Import String List ResultT.
+Require Import JSON Stringifiable.
+Import ListNotations.
+
+Record Attestation_Session := {
+  Session_Plc     : Plc ;
+  Plc_Mapping     : MapC Plc UUID;
+  PubKey_Mapping  : MapC Plc PublicKey;
+}.
+
+Inductive DispatcherErrors : Type :=
+| Unavailable   : DispatcherErrors
+| Runtime       : string -> DispatcherErrors.
+
+Inductive CallBackErrors : Type := 
+| messageLift   : string -> CallBackErrors.
+
+Definition ASPCallback (ErrType : Type) : Type := 
+  ASP_PARAMS -> RawEv -> ResultT RawEv ErrType.
+
+Definition PolicyT := list (Plc * ASP_ID).
+
+Record Session_Config := {
+  session_plc         : Plc ;
+  ASP_to_APPR_ASP_Map : MapC ASP_ID ASP_ID ;
+  aspCb               : (ASPCallback DispatcherErrors) ;
+  plc_map             : MapC Plc UUID ;
+  pubkey_map          : MapC Plc PublicKey ;
+  policy              : PolicyT ;
+}.
+
+Open Scope string_scope.
+Global Instance Jsonifiable_Attestation_Session `{Jsonifiable (MapC Plc UUID), Jsonifiable (MapC Plc PublicKey)}: Jsonifiable Attestation_Session.
+eapply Build_Jsonifiable with 
+  (to_JSON := (fun v => 
+                JSON_Object [
+                  ("Session_Plc", InJSON_String (to_string (Session_Plc v)));
+                  ("Plc_Mapping", InJSON_Object (to_JSON (Plc_Mapping v)));
+                  ("PubKey_Mapping", InJSON_Object (to_JSON (PubKey_Mapping v)))])) 
+  (from_JSON := (fun j =>
+    match (JSON_get_string "Session_Plc" j), (JSON_get_Object "Plc_Mapping" j), (JSON_get_Object "PubKey_Mapping" j) with
+    | resultC plc, resultC plc_map, resultC pub_map =>
+        match (from_string plc), (from_JSON plc_map), (from_JSON pub_map) with
+        | resultC plc', resultC plc_map', resultC pub_map' =>
+            resultC {| Session_Plc := plc'; Plc_Mapping := plc_map'; PubKey_Mapping := pub_map' |}
+        | _, _, _ => errC "Error in parsing Attestation_Session"
+        end
+    | _, _, _ => errC "Error in parsing Attestation_Session"
+    end)).
+simpl in *; intuition.
+repeat rewrite canonical_jsonification; destruct a; eauto.
+Defined.
