src/CvmJson_Interfaces.v
@@ -3,109 +3,9 @@
     
     At the moment, these are too low-level to represent faithfully in the Coq development.   *)
 
-Require Import Term_Defs_Core Term_Defs List JSON Interface_Types ResultT ErrorStringConstants BS Stringifiable.
-Export Interface_Types JSON.
+Require Import Term_Defs_Core Term_Defs List JSON Interface ResultT ErrorStringConstants BS Stringifiable.
+Export Interface JSON.
 Import ListNotations ResultNotation.
-
-(* Protocol Run Section *)
-Definition ProtocolRunRequest_to_JSON (req: ProtocolRunRequest): JSON :=
-  JSON_Object 
-    [(STR_TYPE, (InJSON_String STR_REQUEST));
-    (STR_ACTION, (InJSON_String STR_RUN));
-    (STR_REQ_PLC, (InJSON_String (to_string (prreq_req_plc req))));
-    (STR_TERM, (InJSON_Object (to_JSON (prreq_term req)))); 
-    (STR_RAWEV, (InJSON_Object (to_JSON (prreq_rawev req))))].
-
-Definition JSON_to_ProtocolRunRequest (req : JSON): ResultT ProtocolRunRequest string :=
-  temp_term <- JSON_get_Object STR_TERM req ;;
-  temp_req_plc <- JSON_get_string STR_REQ_PLC req ;;
-  temp_ev <- JSON_get_Object STR_RAWEV req ;;
-
-  term <- from_JSON temp_term ;;
-  req_plc <- from_string temp_req_plc ;;
-  ev <- from_JSON temp_ev ;;
-  resultC (mkPRReq term req_plc ev).
-
-Definition ProtocolRunResponse_to_JSON (resp: ProtocolRunResponse): JSON :=
-  JSON_Object 
-    [(STR_TYPE, (InJSON_String STR_RESPONSE));
-    (STR_ACTION, (InJSON_String STR_RUN));
-    (STR_SUCCESS, (InJSON_Boolean (prresp_success resp)));
-    (STR_PAYLOAD, (InJSON_Object (to_JSON (prresp_ev resp))))].
-
-Definition JSON_to_ProtocolRunResponse (resp : JSON): ResultT ProtocolRunResponse string :=
-  temp_success <- JSON_get_bool STR_SUCCESS resp ;;
-  temp_ev <- JSON_get_Object STR_PAYLOAD resp ;;
-
-  ev <- from_JSON temp_ev ;;
-  resultC (mkPRResp temp_success ev).
-
-(* Protocol Negotiate Section *)
-Definition ProtocolNegotiateRequest_to_JSON (req: ProtocolNegotiateRequest): JSON :=
-  JSON_Object [
-    (STR_TYPE, (InJSON_String STR_REQUEST));
-    (STR_ACTION, (InJSON_String STR_NEGOTIATE)); 
-    (STR_TERM, (InJSON_Object (to_JSON (pnreq_term req))))
-  ].
-
-Definition JSON_to_ProtocolNegotiateRequest (req : JSON): ResultT ProtocolNegotiateRequest string :=
-  temp_term <- JSON_get_Object STR_TERM req ;;
-
-  term <- from_JSON temp_term ;;
-  resultC (mkPNReq term).
-
-Definition ProtocolNegotiateResponse_to_JSON (resp: ProtocolNegotiateResponse): JSON :=
-  JSON_Object [
-    (STR_TYPE, (InJSON_String STR_RESPONSE));
-    (STR_ACTION, (InJSON_String STR_NEGOTIATE)); 
-    (STR_SUCCESS, (InJSON_Boolean (pnresp_success resp)));
-    (STR_PAYLOAD, (InJSON_Object (to_JSON (pnresp_term resp))))
-  ].
-
-Definition JSON_to_ProtocolNegotiateResponse (resp : JSON): ResultT ProtocolNegotiateResponse string :=
-  temp_success <- JSON_get_bool STR_SUCCESS resp ;;
-  temp_term <- JSON_get_Object STR_PAYLOAD resp ;;
-
-  term <- from_JSON temp_term ;;
-  resultC (mkPNResp temp_success term).
-
-(* Protocol Appraise Section *)
-Definition ProtocolAppraiseRequest_to_JSON (req: ProtocolAppraiseRequest): JSON :=
-  JSON_Object [
-    (STR_TYPE, (InJSON_String STR_REQUEST));
-    (STR_ACTION, (InJSON_String STR_APPRAISE));
-    (STR_TERM, (InJSON_Object (to_JSON (pareq_term req))));
-    (STR_REQ_PLC, (InJSON_String (to_string (pareq_plc req))));
-    (STR_EVIDENCE, (InJSON_Object (to_JSON (pareq_evidence req))));
-    (STR_RAWEV, (InJSON_Object (to_JSON (pareq_ev req))))].
-
-Definition JSON_to_ProtocolAppraiseRequest (req : JSON): ResultT ProtocolAppraiseRequest string :=
-  temp_term <- JSON_get_Object STR_TERM req ;;
-  temp_plc <- JSON_get_string STR_REQ_PLC req ;;
-  temp_evidence <- JSON_get_Object STR_EVIDENCE req ;;
-  temp_ev <- JSON_get_Object STR_RAWEV req ;;
-
-  term <- from_JSON temp_term ;;
-  plc <- from_string temp_plc ;;
-  evidence <- from_JSON temp_evidence ;;
-  ev <- from_JSON temp_ev ;;
-  resultC (mkPAReq term plc evidence ev).
-
-Definition ProtocolAppraiseResponse_to_JSON (resp: ProtocolAppraiseResponse): JSON :=
-  JSON_Object [
-    (STR_TYPE, (InJSON_String STR_RESPONSE));
-    (STR_ACTION, (InJSON_String STR_APPRAISE));
-    (STR_SUCCESS, (InJSON_Boolean (paresp_success resp)));
-    (STR_PAYLOAD, (InJSON_Object (to_JSON (paresp_result resp))))
-  ].
-
-Definition JSON_to_ProtocolAppraiseResponse (resp : JSON): 
-    ResultT ProtocolAppraiseResponse string :=
-  temp_success <- JSON_get_bool STR_SUCCESS resp ;;
-  temp_result <- JSON_get_Object STR_PAYLOAD resp ;;
-
-  result <- from_JSON temp_result ;;
-  resultC (mkPAResp temp_success result).
 
 (* AM Protocol Request Section *)
 Definition AM_Protocol_Request_to_JSON (req: AM_Protocol_Requests): JSON :=
@@ -170,48 +70,7 @@ Definition JSON_to_AM_Protocol_Interface (msg : JSON):
   else errC errStr_incorrect_resp_type.
 
 
-(* ASP Run Request Section *)
-Definition ASPRunRequest_to_JSON (req: ASPRunRequest): JSON :=
-  JSON_Object [
-    (STR_TYPE, (InJSON_String STR_REQUEST));
-    (STR_ACTION, (InJSON_String STR_ASP_RUN));
-    (STR_ASP_ID, (InJSON_String (to_string (asprreq_asp_id req))));
-    (STR_ASP_ARGS, (InJSON_Object (to_JSON (asprreq_asp_args req))));
-    (STR_TARG_PLC, (InJSON_String (to_string (asprreq_targ_plc req))));
-    (STR_TARG, (InJSON_String (to_string (asprreq_targ req))));
-    (STR_RAWEV, (InJSON_Object (to_JSON (asprreq_rawev req))))
-  ].
-
-Definition JSON_to_ASPRunRequest (req : JSON): ResultT ASPRunRequest string :=
-  temp_asp_id <- JSON_get_string STR_ASP_ID req ;;
-  temp_asp_args <- JSON_get_Object STR_ASP_ARGS req ;;
-  temp_targ_plc <- JSON_get_string STR_TARG_PLC req ;;
-  temp_targ <- JSON_get_string STR_TARG req ;;
-  temp_ev <- JSON_get_Object STR_RAWEV req ;;
-
-  asp_id <- from_string temp_asp_id ;;
-  asp_args <- from_JSON temp_asp_args ;;
-  targ_plc <- from_string temp_targ_plc ;;
-  targ <- from_string temp_targ ;;
-  ev <- from_JSON temp_ev ;;
-  resultC (mkASPRReq asp_id asp_args targ_plc targ ev).
-
-Definition ASPRunResponse_to_JSON (resp: ASPRunResponse): JSON :=
-  JSON_Object 
-    [(STR_TYPE, (InJSON_String STR_RESPONSE));
-    (STR_ACTION, (InJSON_String STR_ASP_RUN));
-    (STR_SUCCESS, (InJSON_Boolean (asprresp_success resp)));
-    (STR_PAYLOAD, (InJSON_Object (to_JSON (asprresp_rawev resp))))].
-
-Definition JSON_to_ASPRunResponse (resp : JSON): ResultT ASPRunResponse string :=
-  temp_success <- JSON_get_bool STR_SUCCESS resp ;;
-  temp_rawev <- JSON_get_Object STR_PAYLOAD resp ;;
-
-  rawev <- from_JSON temp_rawev ;;
-  resultC (mkASPRResp temp_success rawev).
-
 (* AM ASP Interface Section *)
-
 Definition AM_ASP_Interface_to_JSON (msg: AM_ASP_Interface): JSON :=
   match msg with
   | ASP_Run_Request r => ASPRunRequest_to_JSON r
@@ -233,9 +92,3 @@ Definition JSON_to_AM_ASP_Interface (msg : JSON):
                 resultC (ASP_Run_Response temp_msg))
           else errC errStr_invalid_request_type
   else errC errStr_incorrect_resp_type.
-
-(* Error Response *)
-Definition ErrorResponseJSON (msg: string): JSON :=
-  JSON_Object 
-    [(STR_SUCCESS, InJSON_Boolean false);
-    (STR_PAYLOAD, (InJSON_String msg))].
