src/External_Facts.v
@@ -4,25 +4,25 @@ Axioms and derived lemmas that capture the semantics of external CVM instances.
 Author:  Adam Petz, ampetz@ku.edu
 *)
 
-Require Import Term_Defs Anno_Term_Defs Cvm_St Cvm_Impl Axioms_Io Helpers_CvmSemantics Cvm_Monad ID_Type.
+Require Import Term_Defs Anno_Term_Defs Cvm_St Cvm_Impl Axioms_Io Helpers_CvmSemantics Cvm_Monad ID_Type Attestation_Session.
 
 Require Import List.
 Import ListNotations.
 
 
 (* TODO: This seems obscenely strong!? *)
-Axiom build_cvm_external' : forall (t : Core_Term) (e : EvC) (tr:list Ev) (i:Event_ID) (ac : AM_Config),
+Axiom build_cvm_external' : forall (t : Core_Term) (e : EvC) (tr:list Ev) (i:Event_ID) (ac : Session_Config),
     runErr 
       (build_cvm t)
       {| st_ev := e;
          st_trace := tr;
          st_evid := i;
-         st_AM_config := ac |} =
+         st_config := ac |} =
     (resultC tt,
-     {| st_ev := cvm_evidence_core t (my_abstract_plc (absMan ac)) e;
-        st_trace := tr ++ (cvm_events_core t (my_abstract_plc (absMan ac)) (get_et e));
+     {| st_ev := cvm_evidence_core t (session_plc ac) e;
+        st_trace := tr ++ (cvm_events_core t (session_plc ac) (get_et e));
         st_evid := (i + event_id_span t);
-        st_AM_config := ac
+        st_config := ac
      |}).
 
 Lemma build_cvm_external : forall (t : Core_Term) (e : EvC) i ac,
@@ -30,15 +30,15 @@ Lemma build_cvm_external : forall (t : Core_Term) (e : EvC) i ac,
                     {| st_ev := e;
                        st_trace := [];
                        st_evid := i;
-                       st_AM_config := ac|} =
+                       st_config := ac|} =
     (resultC tt,
-     {| st_ev := cvm_evidence_core t (my_abstract_plc (absMan ac)) e;
-        st_trace := cvm_events_core t (my_abstract_plc (absMan ac)) (get_et e);
+     {| st_ev := cvm_evidence_core t (session_plc ac) e;
+        st_trace := cvm_events_core t (session_plc ac) (get_et e);
         st_evid := (i + event_id_span t);
-        st_AM_config := ac
+        st_config := ac
      |}).
 Proof.
   intros.
-  assert ([] ++ (cvm_events_core t (my_abstract_plc (absMan ac)) (get_et e)) = (cvm_events_core t (my_abstract_plc (absMan ac)) (get_et e))) by eauto.
+  assert ([] ++ (cvm_events_core t (session_plc ac) (get_et e)) = (cvm_events_core t (session_plc ac) (get_et e))) by eauto.
   eapply build_cvm_external'.
 Defined.
