src/Helpers_CvmSemantics.v
@@ -4,22 +4,22 @@ Helper lemmas for proofs about the CVM semantics.
 Author:  Adam Petz, ampetz@ku.edu
 *)
 
-Require Import Anno_Term_Defs Cvm_Monad Cvm_Impl Term_Defs Auto StructTactics AutoApp Manifest ResultT.
+Require Import Anno_Term_Defs Cvm_Monad Cvm_Impl Term_Defs Auto StructTactics AutoApp Attestation_Session ResultT.
 
 Require Import Coq.Program.Tactics Coq.Program.Equality.
 
 Require Import List.
 Import ListNotations.
 
-Lemma ac_immut : forall t e tr i ac,
-  st_AM_config 
+Lemma sc_immut : forall t e tr i ac,
+  st_config 
     (execErr 
       (build_cvm t)
       {|
         st_ev := e;
         st_trace := tr;
         st_evid := i;
-        st_AM_config := ac
+        st_config := ac
       |}) = ac.
 Proof.
   induction t; repeat (monad_unfold; simpl in *); intuition.
@@ -33,43 +33,30 @@ Proof.
     repeat ff.
 
   - pose proof (IHt1 e tr i ac).
-    destruct (build_cvm t1 {| st_ev := e; st_trace := tr; st_evid := i; st_AM_config := ac |}) eqn:C1;
+    destruct (build_cvm t1 {| st_ev := e; st_trace := tr; st_evid := i; st_config := ac |}) eqn:C1;
     simpl in *; eauto;
     destruct r; simpl in *; intuition; eauto.
     destruct c; simpl in *.
-    pose proof (IHt2 st_ev st_trace st_evid st_AM_config).
-    destruct (build_cvm t2 {| st_ev := st_ev; st_trace := st_trace; st_evid := st_evid; st_AM_config := st_AM_config |}) eqn:C2;
+    pose proof (IHt2 st_ev st_trace st_evid st_config).
+    destruct (build_cvm t2 {| st_ev := st_ev; st_trace := st_trace; st_evid := st_evid; st_config := st_config |}) eqn:C2;
     simpl in *; subst; eauto.
   - 
     monad_unfold; simpl in *.
-    pose proof (IHt1 e (tr ++ [Term_Defs.split i (my_abstract_plc (absMan ac))]) (i + 1) ac).
-    destruct (build_cvm t1 {| st_ev := e; st_trace := tr ++ [Term_Defs.split i (my_abstract_plc (absMan ac)) ]; st_evid := (i + 1); st_AM_config := ac |}) eqn:C1;
+    pose proof (IHt1 e (tr ++ [Term_Defs.split i (session_plc ac)]) (i + 1) ac).
+    destruct (build_cvm t1 {| st_ev := e; st_trace := tr ++ [Term_Defs.split i (session_plc ac) ]; st_evid := (i + 1); st_config := ac |}) eqn:C1;
     simpl in *; eauto;
     destruct r; simpl in *; intuition; eauto.
     destruct c; simpl in *.
-    pose proof (IHt2 e st_trace st_evid st_AM_config).
-    destruct (build_cvm t2 {| st_ev := e; st_trace := st_trace; st_evid := st_evid; st_AM_config := st_AM_config |}) eqn:C2;
+    pose proof (IHt2 e st_trace st_evid st_config).
+    destruct (build_cvm t2 {| st_ev := e; st_trace := st_trace; st_evid := st_evid; st_config := st_config |}) eqn:C2;
     simpl in *; subst; eauto;
     destruct r; simpl in *; eauto.
   - monad_unfold; simpl in *.
-    pose proof (IHt1 e ((tr ++ [Term_Defs.split i (my_abstract_plc (absMan ac))]) ++ [cvm_thread_start l (my_abstract_plc (absMan ac)) t2 (get_et e)]) (i + 1) ac).
-    destruct (build_cvm t1 {| st_ev := e; st_trace := (tr ++ [Term_Defs.split i (my_abstract_plc (absMan ac))]) ++ [cvm_thread_start l (my_abstract_plc (absMan ac)) t2 (get_et e)]; st_evid := (i + 1); st_AM_config := ac |}) eqn:C1;
+    pose proof (IHt1 e ((tr ++ [Term_Defs.split i (session_plc ac)]) ++ [cvm_thread_start l (session_plc ac) t2 (get_et e)]) (i + 1) ac).
+    destruct (build_cvm t1 {| st_ev := e; st_trace := (tr ++ [Term_Defs.split i (session_plc ac)]) ++ [cvm_thread_start l (session_plc ac) t2 (get_et e)]; st_evid := (i + 1); st_config := ac |}) eqn:C1;
     simpl in *; eauto;
     destruct r; simpl in *; intuition; eauto.
-    destruct c; simpl in *; eauto.
 Qed.
-
-Lemma st_congr :
-  forall st tr e i ac,
-    st_ev st = e ->
-    st_trace st = tr ->
-    st_evid st = i ->
-    st_AM_config st = ac ->
-    st = {| st_ev := e; st_trace := tr; st_evid := i; st_AM_config := ac |}.
-Proof.
-  intros.
-  subst; destruct st; auto.
-Defined.
 
 (* Hack to apply a specific induction hypothesis in some proofs *)
 Ltac anhl :=
@@ -87,8 +74,8 @@ Ltac monad_simp :=
   repeat (monad_unfold; simpl in *; eauto).
 
 Theorem evidence_deterministic_output_on_results : forall t e tr1 tr2 i1 i2 ac st1 st2,
-  build_cvm t {| st_ev := e; st_trace := tr1; st_evid := i1; st_AM_config := ac |} = (resultC tt, st1) ->
-  build_cvm t {| st_ev := e; st_trace := tr2; st_evid := i2; st_AM_config := ac |} = (resultC tt, st2) ->
+  build_cvm t {| st_ev := e; st_trace := tr1; st_evid := i1; st_config := ac |} = (resultC tt, st1) ->
+  build_cvm t {| st_ev := e; st_trace := tr2; st_evid := i2; st_config := ac |} = (resultC tt, st2) ->
   st1.(st_ev) = st2.(st_ev).
 Proof.
   induction t; intros; monad_simp.
@@ -102,43 +89,43 @@ Proof.
   repeat ff.
   find_rewrite.
   ff.
-  - destruct (build_cvm t1 {| st_ev := e; st_trace := tr1; st_evid := i1; st_AM_config := ac |}) eqn:E1;
-    destruct (build_cvm t1 {| st_ev := e; st_trace := tr2; st_evid := i2; st_AM_config := ac |}) eqn:E2;
+  - destruct (build_cvm t1 {| st_ev := e; st_trace := tr1; st_evid := i1; st_config := ac |}) eqn:E1;
+    destruct (build_cvm t1 {| st_ev := e; st_trace := tr2; st_evid := i2; st_config := ac |}) eqn:E2;
     destruct r, r0; invc H; invc H0; destruct u, u0, c, c0.
     pose proof (IHt1 _ _ _ _ _ _ _ _ E1 E2); simpl in *; subst.
-    assert (st_AM_config = st_AM_config0). {
-      pose proof (ac_immut t1 e tr2 i2 ac); monad_unfold;
-      pose proof (ac_immut t1 e tr1 i1 ac); monad_unfold.
+    assert (st_config = st_config0). {
+      pose proof (sc_immut t1 e tr2 i2 ac); monad_unfold;
+      pose proof (sc_immut t1 e tr1 i1 ac); monad_unfold.
       rewrite E1, E2 in *; simpl in *; subst; eauto.
     }
     subst; clear E1 E2.
-    destruct (build_cvm t2 {| st_ev := st_ev0; st_trace := st_trace; st_evid := st_evid; st_AM_config := st_AM_config0 |}) eqn:E1;
-    destruct (build_cvm t2 {| st_ev := st_ev0; st_trace := st_trace0; st_evid := st_evid0; st_AM_config := st_AM_config0 |}) eqn:E2;
+    destruct (build_cvm t2 {| st_ev := st_ev0; st_trace := st_trace; st_evid := st_evid; st_config := st_config0 |}) eqn:E1;
+    destruct (build_cvm t2 {| st_ev := st_ev0; st_trace := st_trace0; st_evid := st_evid0; st_config := st_config0 |}) eqn:E2;
     invc H1; invc H2; simpl in *; eauto.
-  - destruct (build_cvm t1 {| st_ev := e; st_trace := tr1 ++ [Term_Defs.split i1 (my_abstract_plc (absMan ac))]; st_evid := i1 + 1; st_AM_config := ac |}) eqn:E1;
-    destruct (build_cvm t1 {| st_ev := e; st_trace := tr2 ++ [Term_Defs.split i2 (my_abstract_plc (absMan ac))]; st_evid := i2 + 1; st_AM_config := ac |}) eqn:E2;
+  - destruct (build_cvm t1 {| st_ev := e; st_trace := tr1 ++ [Term_Defs.split i1 (session_plc ac)]; st_evid := i1 + 1; st_config := ac |}) eqn:E1;
+    destruct (build_cvm t1 {| st_ev := e; st_trace := tr2 ++ [Term_Defs.split i2 (session_plc ac)]; st_evid := i2 + 1; st_config := ac |}) eqn:E2;
     destruct r, r0; invc H; invc H0; destruct u, u0, c, c0.
     pose proof (IHt1 _ _ _ _ _ _ _ _ E1 E2); simpl in *; subst.
-    assert (st_AM_config = st_AM_config0). {
-      pose proof (ac_immut t1 e (tr2 ++ [Term_Defs.split i2 (my_abstract_plc (absMan ac))]) (i2 + 1) ac); monad_unfold;
-      pose proof (ac_immut t1 e (tr1 ++ [Term_Defs.split i1 (my_abstract_plc (absMan ac))]) (i1 + 1) ac); monad_unfold;
+    assert (st_config = st_config0). {
+      pose proof (sc_immut t1 e (tr2 ++ [Term_Defs.split i2 (session_plc ac)]) (i2 + 1) ac); monad_unfold;
+      pose proof (sc_immut t1 e (tr1 ++ [Term_Defs.split i1 (session_plc ac)]) (i1 + 1) ac); monad_unfold;
       rewrite E1, E2 in *; simpl in *; subst; eauto.
     }
     subst; clear E1 E2.
-    destruct (build_cvm t2 {| st_ev := e; st_trace := st_trace; st_evid := st_evid; st_AM_config := st_AM_config0 |}) eqn:E1;
-    destruct (build_cvm t2 {| st_ev := e; st_trace := st_trace0; st_evid := st_evid0; st_AM_config := st_AM_config0 |}) eqn:E2;
+    destruct (build_cvm t2 {| st_ev := e; st_trace := st_trace; st_evid := st_evid; st_config := st_config0 |}) eqn:E1;
+    destruct (build_cvm t2 {| st_ev := e; st_trace := st_trace0; st_evid := st_evid0; st_config := st_config0 |}) eqn:E2;
     destruct r0, r;
     invc H1; invc H2; simpl in *;
     destruct u, u0.
     pose proof (IHt2 _ _ _ _ _ _ _ _ E1 E2); simpl in *; subst; 
     rewrite H; eauto.
-  - destruct (build_cvm t1 {| st_ev := e; st_trace := (tr1 ++ [Term_Defs.split i1 (my_abstract_plc (absMan ac))]) ++ [cvm_thread_start l (my_abstract_plc (absMan ac)) t2 (get_et e)]; st_evid := i1 + 1; st_AM_config := ac |}) eqn:E1;
-    destruct (build_cvm t1 {| st_ev := e; st_trace := (tr2 ++ [Term_Defs.split i2 (my_abstract_plc (absMan ac))]) ++ [cvm_thread_start l (my_abstract_plc (absMan ac)) t2 (get_et e)]; st_evid := i2 + 1; st_AM_config := ac |}) eqn:E2;
+  - destruct (build_cvm t1 {| st_ev := e; st_trace := (tr1 ++ [Term_Defs.split i1 (session_plc ac)]) ++ [cvm_thread_start l (session_plc ac) t2 (get_et e)]; st_evid := i1 + 1; st_config := ac |}) eqn:E1;
+    destruct (build_cvm t1 {| st_ev := e; st_trace := (tr2 ++ [Term_Defs.split i2 (session_plc ac)]) ++ [cvm_thread_start l (session_plc ac) t2 (get_et e)]; st_evid := i2 + 1; st_config := ac |}) eqn:E2;
     destruct r, r0; invc H; invc H0; destruct u, u0, c, c0.
     pose proof (IHt1 _ _ _ _ _ _ _ _ E1 E2); simpl in *; subst.
-    assert (st_AM_config = st_AM_config0). {
-      pose proof (ac_immut t1 e ((tr1 ++ [Term_Defs.split i1 (my_abstract_plc (absMan ac))]) ++ [cvm_thread_start l (my_abstract_plc (absMan ac)) t2 (get_et e)]) (i1 + 1) ac); monad_unfold;
-      pose proof (ac_immut t1 e ((tr2 ++ [Term_Defs.split i2 (my_abstract_plc (absMan ac))]) ++ [cvm_thread_start l (my_abstract_plc (absMan ac)) t2 (get_et e)]) (i2 + 1) ac); monad_unfold.
+    assert (st_config = st_config0). {
+      pose proof (sc_immut t1 e ((tr1 ++ [Term_Defs.split i1 (session_plc ac)]) ++ [cvm_thread_start l (session_plc ac) t2 (get_et e)]) (i1 + 1) ac); monad_unfold;
+      pose proof (sc_immut t1 e ((tr2 ++ [Term_Defs.split i2 (session_plc ac)]) ++ [cvm_thread_start l (session_plc ac) t2 (get_et e)]) (i2 + 1) ac); monad_unfold.
       rewrite E1, E2 in *; simpl in *; subst; eauto.
     }
     subst; clear E1 E2; eauto.
@@ -150,7 +137,7 @@ Lemma cvm_errors_deterministic :  forall t e tr1 tr2 i ac r1 r2 st1 st2,
       st_ev := e;
       st_trace := tr1;
       st_evid := i;
-      st_AM_config := ac
+      st_config := ac
     |} =
   (r1, st1) -> 
 
@@ -159,11 +146,11 @@ Lemma cvm_errors_deterministic :  forall t e tr1 tr2 i ac r1 r2 st1 st2,
       st_ev := e;
       st_trace := tr2;
       st_evid := i;
-      st_AM_config := ac
+      st_config := ac
     |} =
   (r2, st2) -> 
 
-  (r1 = r2 /\ st1.(st_ev) = st2.(st_ev) /\ st1.(st_AM_config) = st2.(st_AM_config) /\
+  (r1 = r2 /\ st1.(st_ev) = st2.(st_ev) /\ st1.(st_config) = st2.(st_config) /\
     st1.(st_evid) = st2.(st_evid)).
 Proof.
   induction t; intros; monad_simp.
@@ -209,10 +196,10 @@ Qed.
 (* Lemma stating the following:  If all starting parameters to the cvm_st are the same, except 
    for possibly the trace, then all of those final parameters should also be equal. *)
 Lemma st_trace_irrel : forall t e e' e'' x x' y y' i i' i'' ac ac' ac'' res,
-    build_cvm t {| st_ev := e; st_trace := x; st_evid := i; st_AM_config := ac |} =
-    (res, {| st_ev := e'; st_trace := x'; st_evid := i'; st_AM_config := ac' |}) ->
-    build_cvm t {| st_ev := e; st_trace := y; st_evid := i; st_AM_config := ac |} =
-    (res, {| st_ev := e''; st_trace := y'; st_evid := i''; st_AM_config := ac'' |}) ->
+    build_cvm t {| st_ev := e; st_trace := x; st_evid := i; st_config := ac |} =
+    (res, {| st_ev := e'; st_trace := x'; st_evid := i'; st_config := ac' |}) ->
+    build_cvm t {| st_ev := e; st_trace := y; st_evid := i; st_config := ac |} =
+    (res, {| st_ev := e''; st_trace := y'; st_evid := i''; st_config := ac'' |}) ->
     (e' = e'' /\ i' = i'' /\ ac' = ac'').
 Proof.
   intros; find_eapply_lem_hyp cvm_errors_deterministic; 
@@ -224,10 +211,10 @@ Ltac dohi'' :=
   annogo;
   let tac H H' := eapply st_trace_irrel; [apply H | apply H'] in
   match goal with
-  | [H : build_cvm ?t1 {| st_ev := ?e; st_trace := _; st_evid := ?i; st_AM_config := ?ac |} =
-         (?opt, {| st_ev := ?e'; st_trace := _; st_evid := ?i'; st_AM_config := ?ac' |}),
-         H' : build_cvm ?t1 {| st_ev := ?e; st_trace := _; st_evid := ?i; st_AM_config := ?ac |} =
-              (?opt, {| st_ev := ?e''; st_trace := _; st_evid := ?i''; st_AM_config := ?ac'' |})
+  | [H : build_cvm ?t1 {| st_ev := ?e; st_trace := _; st_evid := ?i; st_config := ?ac |} =
+         (?opt, {| st_ev := ?e'; st_trace := _; st_evid := ?i'; st_config := ?ac' |}),
+         H' : build_cvm ?t1 {| st_ev := ?e; st_trace := _; st_evid := ?i; st_config := ?ac |} =
+              (?opt, {| st_ev := ?e''; st_trace := _; st_evid := ?i''; st_config := ?ac'' |})
      |- _] =>
     assert_new_proof_by (e' = e'' /\ i' = i'' /\ ac' = ac'') ltac:(tac H H')
   end.
@@ -240,16 +227,16 @@ Ltac dohi :=
    This is a simple corollary of the Lemma hihi above. *)
 Lemma trace_irrel_ev : forall t tr1 tr1' tr2 e e' i i' ac ac' res,
     build_cvm t
-           {| st_ev := e; st_trace := tr1; st_evid := i; st_AM_config := ac |} =
-    (res, {| st_ev := e'; st_trace := tr1'; st_evid := i'; st_AM_config := ac' |}) ->
+           {| st_ev := e; st_trace := tr1; st_evid := i; st_config := ac |} =
+    (res, {| st_ev := e'; st_trace := tr1'; st_evid := i'; st_config := ac' |}) ->
     
     st_ev
       (execErr (build_cvm t)
-           {| st_ev := e; st_trace := tr2; st_evid := i; st_AM_config := ac |}) = e'.
+           {| st_ev := e; st_trace := tr2; st_evid := i; st_config := ac |}) = e'.
 Proof.
 
 intros.
-destruct (build_cvm t {| st_ev := e; st_trace := tr2; st_evid := i; st_AM_config := ac |}) eqn:ff.
+destruct (build_cvm t {| st_ev := e; st_trace := tr2; st_evid := i; st_config := ac |}) eqn:ff.
 simpl.
 vmsts.
 simpl.
@@ -275,16 +262,16 @@ Defined.
    This is a simple corollary of the Lemma hihi above. *)
 Lemma trace_irrel_evid : forall t tr1 tr1' tr2 e e' i i' ac ac' res,
     build_cvm t
-           {| st_ev := e; st_trace := tr1; st_evid := i; st_AM_config := ac|} =
-    (res, {| st_ev := e'; st_trace := tr1'; st_evid := i'; st_AM_config := ac' |}) ->
+           {| st_ev := e; st_trace := tr1; st_evid := i; st_config := ac|} =
+    (res, {| st_ev := e'; st_trace := tr1'; st_evid := i'; st_config := ac' |}) ->
     
     st_evid
       (execErr (build_cvm t)
-           {| st_ev := e; st_trace := tr2; st_evid := i; st_AM_config := ac |}) = i'.
+           {| st_ev := e; st_trace := tr2; st_evid := i; st_config := ac |}) = i'.
 Proof.
 
 intros.
-destruct (build_cvm t {| st_ev := e; st_trace := tr2; st_evid := i; st_AM_config := ac |}) eqn:ff.
+destruct (build_cvm t {| st_ev := e; st_trace := tr2; st_evid := i; st_config := ac |}) eqn:ff.
 simpl.
 vmsts.
 simpl.
@@ -311,15 +298,15 @@ Defined.
    This is a simple corollary of the Lemma hihi above. *)
 Lemma trace_irrel_ac : forall t tr1 tr1' tr2 e e' i i' ac ac' res,
     build_cvm t
-           {| st_ev := e; st_trace := tr1; st_evid := i; st_AM_config := ac |} =
-    (res, {| st_ev := e'; st_trace := tr1'; st_evid := i'; st_AM_config := ac' |}) ->
+           {| st_ev := e; st_trace := tr1; st_evid := i; st_config := ac |} =
+    (res, {| st_ev := e'; st_trace := tr1'; st_evid := i'; st_config := ac' |}) ->
     
-    st_AM_config
+    st_config
       (execErr (build_cvm t)
-           {| st_ev := e; st_trace := tr2; st_evid := i; st_AM_config := ac |}) = ac'.
+           {| st_ev := e; st_trace := tr2; st_evid := i; st_config := ac |}) = ac'.
 Proof.
   intros.
-  destruct (build_cvm t {| st_ev := e; st_trace := tr2; st_evid := i; st_AM_config := ac |}) eqn:ff.
+  destruct (build_cvm t {| st_ev := e; st_trace := tr2; st_evid := i; st_config := ac |}) eqn:ff.
   simpl.
   vmsts.
   simpl.
@@ -343,19 +330,19 @@ Defined.
 
 Ltac do_st_trace :=
   match goal with
-  | [H': context[{| st_ev := ?e; st_trace := ?tr; st_evid := ?i; st_AM_config := ?ac |}]
+  | [H': context[{| st_ev := ?e; st_trace := ?tr; st_evid := ?i; st_config := ?ac |}]
      |- context[?tr]] =>
     assert_new_proof_by
-      (tr = st_trace {| st_ev := e; st_trace := tr; st_evid := i; st_AM_config := ac |} )
+      (tr = st_trace {| st_ev := e; st_trace := tr; st_evid := i; st_config := ac |} )
       tauto
   end.
 
 Ltac do_st_trace_assumps :=
   match goal with
-  | [H': context[{| st_ev := ?e; st_trace := ?tr; st_evid := ?i; st_AM_config := ?ac |}]
+  | [H': context[{| st_ev := ?e; st_trace := ?tr; st_evid := ?i; st_config := ?ac |}]
      |- _] =>
     assert_new_proof_by
-      (tr = st_trace {| st_ev := e; st_trace := tr; st_evid := i; st_AM_config := ac |} )
+      (tr = st_trace {| st_ev := e; st_trace := tr; st_evid := i; st_config := ac |} )
       tauto
   end.
 
@@ -512,10 +499,10 @@ Ltac wrap_ccp_anno :=
 Ltac cumul_ih :=
   match goal with
   | [H: context[(st_trace _ = _ ++ st_trace _)],
-        H': build_cvmP ?t1 {| st_ev := _; st_trace := ?m ++ ?k; st_evid := _; st_AM_config := _ |}
+        H': build_cvmP ?t1 {| st_ev := _; st_trace := ?m ++ ?k; st_evid := _; st_config := _ |}
                              (?res)
                              ?v_full,
-            H'': build_cvmP ?t1 {| st_ev := _; st_trace := ?k; st_evid := _; st_AM_config := _ |}
+            H'': build_cvmP ?t1 {| st_ev := _; st_trace := ?k; st_evid := _; st_config := _ |}
                                   (?res)
                                   ?v_suffix
      |- _] =>
