src/Server_AM.v
@@ -1,12 +1,15 @@
 (*  Implementation of a top-level Server (listener) thread for Server AMs in
       end-to-end Copland Attestation + Appraisal protocols.  *)
-Require Import String BS Manifest CvmJson_Interfaces AM_Helpers AM_Json_Interfaces.
+Require Import String BS Attestation_Session Interface AM_Helpers AM_Json_Interfaces.
 Require Import List ResultT.
 Import ListNotations.
 Open Scope string_scope.
 
-Definition handle_AM_request (s:string) (ac : AM_Config) (nonceVal:BS) : string :=
+Definition handle_AM_request (s:string) (sc : Session_Config) 
+    (nonceVal:BS) : string :=
   match string_to_JSON s with
   | errC msg => JSON_to_string (ErrorResponseJSON msg)
-  | resultC js => JSON_to_string (handle_AM_request_JSON js ac nonceVal)
+  | resultC js => JSON_to_string (handle_AM_request_JSON js sc nonceVal)
   end.
+
+
