src/Session_Config_Compiler.v
@@ -1,0 +1,51 @@
+Require Import Manifest Attestation_Session.
+Require Import EqClass.
+Require Import Term_Defs_Core ResultT ID_Type Manifest_Set Maps Interface.
+Require Import IO_Stubs.
+
+Definition generate_ASP_dispatcher' (am : Manifest) (ats : Attestation_Session) (aspBin : FS_Location) (par : ASP_PARAMS) (rawEv : RawEv) : ResultT RawEv DispatcherErrors :=
+  let (aspid, args, targ_plc, targ) := par in
+  let asps := am.(asps) in
+  let asp_map := am.(ASP_Mapping) in
+    (* check is the ASPID is available *) 
+    if (in_dec_set aspid asps)
+    then 
+      match (map_get asp_map aspid) with
+      | Some conc_asp_loc => 
+          let asp_req := (mkASPRReq aspid args targ_plc targ rawEv) in
+          let js_req := to_JSON asp_req in
+          let resp_res := make_JSON_FS_Location_Request aspBin conc_asp_loc js_req in
+          match resp_res with
+          | resultC js_resp =>
+              match from_JSON js_resp with
+              | resultC r => 
+                  let '(mkASPRResp succ bs) := r in
+                  resultC bs
+              | errC msg => errC (Runtime msg)
+              end
+          | errC msg => errC (Runtime msg)
+          end
+      | None => errC Unavailable
+      end
+    else errC Unavailable.
+
+(* This function will be a dispatcher for either local ASPS to CakeMLCallback, or pass them off to the ASP_Server *)
+Definition generate_ASP_dispatcher `{HID : EqClass ID_Type} (am : Manifest) (al : Attestation_Session) (aspBin : FS_Location) 
+    : (ASPCallback DispatcherErrors) :=
+  (generate_ASP_dispatcher' am al aspBin). 
+
+Definition session_config_compiler (m : Manifest) (aspBin : FS_Location) (ats : Attestation_Session) : Session_Config :=
+{|
+  session_plc := (Session_Plc ats) ;
+  ASP_to_APPR_ASP_Map := (ASP_Compat_Map m);
+  aspCb     := (generate_ASP_dispatcher m ats aspBin) ;
+  plc_map     := (Plc_Mapping ats);
+  pubkey_map  := (PubKey_Mapping ats);
+  policy   := (man_policy m);
+|}.
+
+Definition session_config_decompiler (sc : Session_Config) : Attestation_Session :=
+{|
+  Session_Plc := (session_plc sc) ;
+  Plc_Mapping := (plc_map sc) ;
+  PubKey_Mapping := (pubkey_map sc) |}.
